src/FJ/RefinementTable.v
@@ -4,22 +4,13 @@ Require Import FJ.Syntax.
 Require Import FJ.ClassTable.
 
 (* A fixed Refinement Table*)
-Parameter RT: ClassRefinement -> RefinementName.
-
-Definition isRefinement (C: Class): bool:=
-  match C with
-  | CD _ => false
-  | CR _ => true
-  end.
-
-Definition RefT := filter isRefinement CT.
-
+Parameter RT: [ClassRefinement].
 
 Inductive succ (C: Class) (C': ClassRefinement): Prop :=
-  | S_Decl : forall C1 C2 D fs K noDupfs mds noDupMds ft fs' nodupfs' K' mds' noDupMds',
-    C = CD (CDecl C1 D fs noDupfs K mds noDupMds ) ->
-    C' = (CRefine C2 ft fs' nodupfs' K' mds' noDupMds') ->
-    find (ref C) RefT = Some (CR (CRefine C2 ft fs' nodupfs' K' mds' noDupMds')) ->
+  | S_Decl : forall C1 C2 D fs K noDupfs mds noDupMds ft fs' nodupfs' K' mds' noDupMds' mdrs noDupMdrs,
+    C = CD (CDecl C1 D fs noDupfs K mds noDupMds) ->
+    C' = CRefine C2 ft fs' nodupfs' K' mds' noDupMds' mdrs noDupMdrs ->
+    find C1 RT = Some C' ->
     succ C C'.
 
 Fixpoint suc (C: ClassName) ft ct : option ClassRefinement :=
@@ -28,15 +19,10 @@ Fixpoint suc (C: ClassName) ft ct : option ClassRefinement :=
   | c :: cs => 
    match c with 
     | CD _ => suc C ft cs
-    | CR ((CRefine C' ft' _ _ _ _ _) as CRef) => 
+    | CR ((CRefine C' ft' _ _ _ _ _ _ _) as CRef) => 
      match beq_id C C' with
       | true => if lt_dec ft ft' then Some CRef else suc C ft cs
       | false => suc C ft cs
      end
    end
   end.
-
-Definition succ (C: Class) : option ClassRefinement :=
-  match C with
-  | CD CDec => suc (ref CDec) 0 CT
-  | CR (CRefi
